capturing more invariants on EqGraph - equivalence classes decrease after a merge - each of the nodes have a unique type
These may be useful for proving termination for
`Ppcc.EqGraph.process_equation`

Core/Ppcc/Basic.lean
@@ -300,11 +300,77 @@ def Term.appc (KA KB : Kind): Term :=
         (.cast ((t#4 • t#2) ~[KB]~ (t#0 • t#1)) #1                           -- A • C ~ B • D
         (.cast ((t#4 • t#2) ~[KB]~ (t#4 • t#0)) #0 (refl! (t#3 • t#1))))
 
-def EqGraph.appc (G : GlobalEnv) (Δ : KindEnv) (Γ : TyEnv) (t1 t2 : Term) (KA KB : Kind) (A1 A2 B1 B2 : Ty)
+def EqGraph.appc (G : GlobalEnv) (wf : ⊢ G) (Δ : KindEnv) (Γ : TyEnv) (t1 t2 : Term) (KA KB : Kind) (A1 A2 B1 B2 : Ty)
   (j1 : (G&Δ, Γ ⊢ t1 : (A1 ~[KA -:> KB]~ A2))) (j2 : (G&Δ, Γ ⊢ t2 : (B1 ~[KA]~ B2))) :
   ((t : Term) ×' (G&Δ, Γ ⊢ t : ((A1 • B1) ~[KB]~ (A2 • B2)))) :=
   ⟨(((((Term.appc KA KB •[A1]) •[A2]) •[B1]) •[B2]) • t1) • t2,
-   by sorry⟩
+   by have lem1 := terms_have_star_types wf j1
+      have lem2 := terms_have_star_types wf j2
+      cases lem1; case _ jA1 jA2 =>
+      cases lem2; case _ jB1 jB2 =>
+      apply Typing.app (A := B1 ~[KA]~ B2)
+      · apply Typing.app (A := (A1 ~[KA -:> KB]~ A2))
+        · apply Typing.appt (K := KA)
+                (P := (A1⟨Ren.succ Ty⟩ ~[KA -:> KB]~ A2⟨Ren.succ Ty⟩) -:> (B1⟨Ren.succ Ty⟩ ~[KA]~ t#0) -:> ((A1⟨Ren.succ Ty⟩ • B1⟨Ren.succ Ty⟩) ~[KB]~ (A2⟨Ren.succ Ty⟩ • t#0)))
+          · apply Typing.appt (K := KA)
+                (P := ∀[KA](A1⟨Ren.succ Ty⟩⟨Ren.succ Ty⟩ ~[KA -:> KB]~ A2⟨Ren.succ Ty⟩⟨Ren.succ Ty⟩) -:> (t#1 ~[KA]~ t#0) -:> ((A1⟨Ren.succ Ty⟩⟨Ren.succ Ty⟩ • t#1) ~[KB]~ (A2⟨Ren.succ Ty⟩⟨Ren.succ Ty⟩ • t#0)))
+            · apply Typing.appt (K := KA -:> KB)
+                (P := ∀[KA]∀[KA](A1⟨Ren.succ Ty⟩⟨Ren.succ Ty⟩⟨Ren.succ Ty⟩ ~[KA -:> KB]~ t#2) -:> (t#1 ~[KA]~ t#0) -:> ((A1⟨Ren.succ Ty⟩⟨Ren.succ Ty⟩⟨Ren.succ Ty⟩ • t#1) ~[KB]~ (t#2 • t#0)))
+              · apply Typing.appt (K := KA -:> KB)
+                 (P := ∀[KA -:> KB]∀[KA]∀[KA](t#3 ~[KA -:> KB]~ t#2) -:> ((t#1 ~[KA]~ t#0) -:> ((t#3 • t#1) ~[KB]~ (t#2 • t#0))))
+                · simp only [Term.appc];
+                  apply Typing.lamt
+                  · apply Kinding.all; apply Kinding.all; apply Kinding.all; apply Kinding.all; apply Kinding.arrow;
+                    · apply Kinding.eq <;> (apply Kinding.var; simp)
+                    · apply Kinding.arrow
+                      · apply Kinding.eq <;> (apply Kinding.var; simp)
+                      · apply Kinding.eq <;> (apply Kinding.app (A := KA); repeat (apply Kinding.var; simp))
+                  · apply Typing.lamt
+                    · apply Kinding.all; apply Kinding.all; apply Kinding.all; apply Kinding.arrow;
+                      · apply Kinding.eq <;> (apply Kinding.var; simp)
+                      · apply Kinding.arrow
+                        · apply Kinding.eq <;> (apply Kinding.var; simp)
+                        · apply Kinding.eq <;> (apply Kinding.app (A := KA); repeat (apply Kinding.var; simp))
+                    · apply Typing.lamt
+                      · apply Kinding.all; apply Kinding.all; apply Kinding.arrow;
+                        · apply Kinding.eq <;> (apply Kinding.var; simp)
+                        · apply Kinding.arrow;
+                          · apply Kinding.eq <;> (apply Kinding.var; simp)
+                          · apply Kinding.eq <;> (apply Kinding.app (A := KA); repeat (apply Kinding.var; simp))
+                      · apply Typing.lamt
+                        · apply Kinding.all; apply Kinding.arrow;
+                          · apply Kinding.eq <;> (apply Kinding.var; simp)
+                          · apply Kinding.arrow;
+                            · apply Kinding.eq <;> (apply Kinding.var; simp)
+                            · apply Kinding.eq <;> (apply Kinding.app (A := KA); repeat (apply Kinding.var; simp))
+                        · apply Typing.lam
+                          · apply Kinding.eq <;> (apply Kinding.var; simp)
+                          · apply Typing.lam
+                            · apply Kinding.eq <;> (apply Kinding.var; simp)
+                            · apply Typing.cast (K := KA -:> KB) (A := t#3) (B := t#2)
+                              · apply Kinding.eq <;> (apply Kinding.app (A := KA); repeat (apply Kinding.var; simp))
+                              · apply Typing.var
+                                · simp
+                                · apply Kinding.eq <;> (apply Kinding.var; simp)
+                              · apply Typing.cast (K := KA) (A := t#1) (B := t#0)
+                                · apply Kinding.eq <;> (apply Kinding.app (A := KA); repeat (apply Kinding.var; simp))
+                                · apply Typing.var
+                                  · simp
+                                  · apply Kinding.eq; repeat (apply Kinding.var; simp)
+                                · simp; apply Typing.refl
+                                  · apply Kinding.app (A := KA); repeat (apply Kinding.var; simp)
+                                · simp
+                              · simp
+                · apply jA1
+                · simp
+              · apply jA2
+              · rw[Ty.subst_all, Ty.subst_all, Ty.subst_arr, Ty.subst_arr, Ty.subst_eq, Ty.subst_eq, Ty.subst_eq, Ty.subst_app, Ty.subst_app, succ_succ_succ_subst_lemma]; simp
+            · apply jB1
+            · rw[Ty.subst_all, Ty.subst_arr, Ty.subst_arr, Ty.subst_eq, Ty.subst_eq, Ty.subst_eq, Ty.subst_app, Ty.subst_app, succ_succ_subst_lemma, succ_succ_subst_lemma]; simp
+          · apply jB2
+          · simp
+        · apply j1
+      · apply j2 ⟩
 
 
 
@@ -362,6 +428,7 @@ instance {G : GlobalEnv} {Δ : KindEnv} {Γ : TyEnv} : Repr (EqGraphNode G Δ Γ
 
 structure EqGraph (G : GlobalEnv) (Δ : KindEnv) (Γ : TyEnv) where
   nodes : List (EqGraphNode G Δ Γ)
+  equiv_class_count : Nat
 
   /-- Validity for parent nodes -/
   -- parent index is less than the length of the nodes
@@ -375,8 +442,10 @@ structure EqGraph (G : GlobalEnv) (Δ : KindEnv) (Γ : TyEnv) where
   /-- all the nodes a unique -/
   unique_nodes : ∀{i j}, (hi : i < nodes.length) -> (hj : j < nodes.length) -> i ≠ j -> nodes[i].ty ≠ nodes[j].ty
 
-  /-- number of equiv classes -/
-  -- equiv_class_count : (nodes.filter (λ n => n.parent_ty == n.ty)).length ≤ nodes.length
+  /-- number of equiv classes min bound -/
+  /-equiv_class_count_ub : nodes.length > 0 -> equiv_class_count ≤ nodes.length
+  equiv_class_count_lb : nodes.length > 0 -> equiv_class_count > 0 -/
+
 
 instance {G : GlobalEnv} {Δ : KindEnv} {Γ : TyEnv} : Repr (EqGraph  G Δ Γ) where
   reprPrec g _ := g.nodes.repr 0
@@ -388,10 +457,13 @@ def EqGraph.elem_node {G : GlobalEnv} {Δ : KindEnv} {Γ : TyEnv} (n : Node G Δ
   List.elem n.ty (eG.nodes.map (λ n => n.ty))
 
 def EqGraph.empty {G : GlobalEnv} {Δ : KindEnv} {Γ : TyEnv} : EqGraph G Δ Γ
-  := { nodes := [], parent_lt := nofun, parent_idx_lt := nofun, parent_kind_eq := nofun, unique_nodes := nofun }
+  := { nodes := [], equiv_class_count := 0, parent_lt := nofun, parent_idx_lt := nofun, parent_kind_eq := nofun
+     , unique_nodes := nofun
+     /-, equiv_class_count_ub := nofun
+     , equiv_class_count_lb := nofun-/ }
 
 def EqGraph.push {G : GlobalEnv} {Δ : KindEnv} {Γ : TyEnv}(eG : EqGraph G Δ Γ) (n : Node G Δ) : EqGraph G Δ Γ :=
-  if eG.elem_node n
+  if h : eG.elem_node n
   then eG
   else let new_node := {
          parent := (eG.nodes.length, n.ty, n.kind),
@@ -399,6 +471,7 @@ def EqGraph.push {G : GlobalEnv} {Δ : KindEnv} {Γ : TyEnv}(eG : EqGraph G Δ �
          parent_rel := ⟨refl! n.ty, by apply Typing.refl; apply n.payload.2.2⟩
          }
        { nodes := eG.nodes ++ [new_node]
+       , equiv_class_count := eG.equiv_class_count + 1
        , parent_lt := by
           intro i h1;
           simp;
@@ -427,7 +500,35 @@ def EqGraph.push {G : GlobalEnv} {Δ : KindEnv} {Γ : TyEnv}(eG : EqGraph G Δ �
             case _ h =>
               have lem : i = eG.nodes.length := by rw[List.length_append] at h1; simp at h1; omega
               subst i; simp[new_node]; congr; simp; simp
-        , unique_nodes := by sorry
+        , unique_nodes := by
+          intro i_idx j_idx hi hj ne
+
+          cases Nat.decLt i_idx eG.nodes.length
+          case _ =>
+            have lemi : i_idx = eG.nodes.length := by simp at hi; omega
+            subst lemi; simp;
+            cases Nat.decLt j_idx eG.nodes.length
+            case _ =>
+              have lemj : j_idx = eG.nodes.length := by simp at hj; omega
+              subst lemj; simp; omega
+            case _ =>
+              rw[List.getElem_append_left (by grind)]; simp [elem_node] at h;
+              replace h := h (eG.nodes[j_idx]) (by simp)
+              simp [new_node]; intro hi; apply h; symm at hi; apply hi
+          case _ =>
+            rw[List.getElem_append_left (by grind)]
+            cases Nat.decLt j_idx eG.nodes.length
+            case _ h =>
+              have lemj : j_idx = eG.nodes.length := by simp at hj; omega
+              subst lemj; simp; clear h;
+              simp [elem_node] at h; replace h := h eG.nodes[i_idx] (by simp);
+              intro hi; rw[hi] at h; simp [new_node] at h
+            case _ =>
+              rw[List.getElem_append_left (by grind)];
+              apply eG.unique_nodes
+              apply ne
+        /-, equiv_class_count_ub := by sorry
+        , equiv_class_count_lb := by simp-/
         }
 
 /-- create an eq class for all the subterms of the type T -/
@@ -499,33 +600,23 @@ def EqGraph.get_eq_class {G : GlobalEnv} {Δ : KindEnv} {Γ : TyEnv} (wf : ⊢ G
     | none => false)
   | none => []
 
-private def EqGraph.check_same_rep {G : GlobalEnv} {Δ : KindEnv} {Γ : TyEnv} {wf : ⊢ G} (eG : EqGraph G Δ Γ)  (T1 : Ty) (T2 : Ty) :
-  Option Unit := do
-  let ⟨ip1, rep_T1, K1, η1, j1⟩ <- eG.get_rep wf T1 -- Maybe • 3
-  let ⟨ip2, rep_T2, K2, η2, j2⟩ <- eG.get_rep wf T2 -- Maybe • 1
-  if ip1 == ip2 && rep_T1 == rep_T2
-  then none
-  else return ()
-
-
-
 
 /-- Merges two equivalence classes for given types, if they belong to the same class it fails -/
-def EqGraph.union {G : GlobalEnv} {Δ : KindEnv} {Γ : TyEnv} {wf : ⊢ G} (eG : EqGraph G Δ Γ) (K : Kind)
+def EqGraph.union {G : GlobalEnv} {Δ : KindEnv} {Γ : TyEnv} (wf : ⊢ G) (eG : EqGraph G Δ Γ) (K : Kind)
   (T1 : Ty) (T2 : Ty) (t : Term) (j : G&Δ, Γ ⊢ t : (T1 ~[K]~ T2)) : Option (EqGraph G Δ Γ) := do
   let i1 <- eG.nodes.findIdx? (·.ty == T1) -- Maybe • 3
   let i2 <- eG.nodes.findIdx? (·.ty == T2) -- 6
-  match eG.nodes[i1]?, eG.nodes[i2]? with
+  match h1 : eG.nodes[i1]?, h2 : eG.nodes[i2]? with
   | some n1, some n2 => do
     let ⟨ip1, rep_T1, K1, η1, j1⟩ <- eG.get_rep wf T1 -- Maybe • 3
     let ⟨ip2, rep_T2, K2, η2, j2⟩ <- eG.get_rep wf T2 -- Maybe • 1
-    let p1n <- eG.nodes[ip1]?
-    let p2n <- eG.nodes[ip2]?
+    match h3 : eG.nodes[ip1]?, h4 : eG.nodes[ip2]? with
+    | some p1n, some p2n =>
     if ip1 == ip2
     then none -- both T1 and T2 are already in the same eq class should never happen
     else
       if h : ip1 < ip2 && (ip2 < eG.nodes.length && (K1 == K2 && (n2.kind == K1 && (n1.kind == K1
-         && (K == K1 && (p1n.ty == rep_T1 && (p1n.kind == K1 && (p2n.ty == rep_T2 && p2n.kind == K2))))))))
+         && (K == K1 && (p1n.ty == rep_T1 && (p1n.kind == K1 && (p2n.ty == rep_T2 && (p2n.kind == K2 && rep_T1 != rep_T2)))))))))
       then
         -- pT2 == T2 == T1 == pT1
         -- symm η2 ; (symm t ; η1)
@@ -536,13 +627,14 @@ def EqGraph.union {G : GlobalEnv} {Δ : KindEnv} {Γ : TyEnv} {wf : ⊢ G} (eG :
             let ⟨symm_t, j'⟩ := EqGraph.symm G wf Δ Γ t K T1 T2 j
             let ⟨symm_η2, j2'⟩ := EqGraph.symm G wf Δ Γ η2 K2 T2 rep_T2 j2
             let ⟨symm_t_η1, j⟩ := EqGraph.seq G wf Δ Γ symm_t η1 K T2 T1 rep_T1 j'
-                         (by simp at h; rcases h with ⟨e1, e2, e3, e4, e5, e6, e7, e8, e9, e10⟩; subst e5; subst e6; apply j1)
+                         (by simp at h; rcases h with ⟨e1, e2, e3, e4, e5, e6, e7, e8, e9, e10, ne11⟩; subst e5; subst e6; apply j1)
             let ⟨symm_η2_symm_t_η1, j⟩ := EqGraph.seq G wf Δ Γ symm_η2 symm_t_η1 K2 rep_T2 T2 rep_T1 j2'
                          (by simp at h; rcases h with ⟨e1, e2, e3, e4, e5, e6, e7, e8, e9, e10⟩; subst e5; subst e6; subst e3; apply j)
             ⟨symm_η2_symm_t_η1, by
               simp at h; rcases h with ⟨e1, e2, e3, e4, e5, e6, e7, e8, e9, e10⟩; subst e5; subst e6; subst e3
               simp only [Node.ty, e10, Node.kind, e9]; apply j⟩ }
         some { nodes := eG.nodes.set ip2 new_node
+             , equiv_class_count := eG.equiv_class_count - 1
              , parent_lt := by
                  intro i h1;
                  simp at h; rcases h with ⟨e1, e2, e3, e4, e5, e6, e7, e8, e9, e10⟩; subst e5; subst e6; subst e3
@@ -575,14 +667,38 @@ def EqGraph.union {G : GlobalEnv} {Δ : KindEnv} {Γ : TyEnv} {wf : ⊢ G} (eG :
                    rcases h with ⟨n, h', e11⟩
                    rw[<-e11]; apply eG.parent_kind_eq
                   case inr h' => rw[h']; simp only [new_node, e10]
-             , unique_nodes := by sorry
+             , unique_nodes := by
+                intro i_idx j_idx hi hj ne
+                rw[List.getElem?_eq_some_iff] at h3 h4;
+                rcases h3 with ⟨_, h3⟩; rcases h4 with ⟨_, h4⟩
+                have ih := @eG.unique_nodes i_idx j_idx (by grind) (by grind) ne
+                have lemi := List.getElem_set hi
+                have lemj := List.getElem_set hj
+                simp at h; rcases h with ⟨e1, e2, e3, e4, e5, e6, e7, e8, e9, e10⟩; subst e5; subst e6; subst e3
+                cases Nat.decEq ip2 i_idx
+                case _ ni =>
+                  cases Nat.decEq ip2 j_idx
+                  case _ nj =>
+                    rw[ite_cond_eq_false (h := by grind)] at lemi
+                    rw[ite_cond_eq_false (h := by grind)] at lemj
+                    rw[lemi, lemj]; apply ih
+                  case _ nj =>
+                    rw[ite_cond_eq_false (h := by grind)] at lemi
+                    rw[ite_cond_eq_true (h := by grind)] at lemj
+                    subst nj; rw[lemj, lemi]; simp only [new_node, EqGraphNode.ty]; rw[h4] at ih
+                    apply ih
+                case _ ni =>
+                  subst ni;
+                  rw[ite_cond_eq_true (h := by grind)] at lemi
+                  rw[ite_cond_eq_false (h := by grind)] at lemj
+                  rw[lemi, lemj]; simp only [new_node, EqGraphNode.ty]; rw[h4] at ih; apply ih
+             /-, equiv_class_count_ub := by
+                sorry
+             , equiv_class_count_lb := by sorry -/
              }
 
-      -- TODO : Perform deduction i.e. if pT1 = A1 • B1, and pT2 = A2 • B2
-      -- then add A1 ~ A2 in the same equiv class and B1 B2 in same equiv class
-
       else if h : ip2 < ip1 && (ip1 < eG.nodes.length && (K1 == K2 && (n2.kind == K1 && (n1.kind == K1
-              && (K == K1 && (p1n.ty == rep_T1 && (p1n.kind == K1 && (p2n.ty == rep_T2 && p2n.kind == K2))))))))
+              && (K == K1 && (p1n.ty == rep_T1 && (p1n.kind == K1 && (p2n.ty == rep_T2 && (p2n.kind == K2 && rep_T1 != rep_T2)))))))))
         then
         -- pT1 == T1 == T2 == pT2
         -- sym η1 ; t ; η2
@@ -601,6 +717,7 @@ def EqGraph.union {G : GlobalEnv} {Δ : KindEnv} {Γ : TyEnv} {wf : ⊢ G} (eG :
               simp at h; rcases h with ⟨e1, e2, e3, e4, e5, e6, e7, e8, e9, e10⟩; subst e5; subst e6; subst e9; subst e3;
               simp only [Node.ty, Node.kind, e8, e7]; apply j⟩ }
          some { nodes := eG.nodes.set ip1 new_node
+              , equiv_class_count := eG.equiv_class_count - 1
               , parent_lt := by
                   intro i h1;
                   simp at h; rcases h with ⟨e1, e2, e3, e4, e5, e6, e7, e8, e9, e10⟩; subst e5; subst e6; subst e9; subst e3
@@ -635,22 +752,41 @@ def EqGraph.union {G : GlobalEnv} {Δ : KindEnv} {Γ : TyEnv} {wf : ⊢ G} (eG :
                    rw[<-e11]; apply eG.parent_kind_eq
                   case inr h' => rw[h']; simp only [new_node, e8]
               , unique_nodes := by
-                 intro i j hi hj ne
-                 simp at h; rcases h with ⟨e1, e2, e3, e4, e5, e6, e7, e8, e9, e10⟩; subst e5; subst e6; subst e9; subst e3
-                 have lem := List.unique_set_unique (l := eG.nodes) (p := ip1) (a := new_node) (by grind) (by grind) (by grind) ne
-                 sorry
+                 intro i_idx j_idx hi hj ne
+                 rw[List.getElem?_eq_some_iff] at h3 h4;
+                 rcases h3 with ⟨_, h3⟩; rcases h4 with ⟨_, h4⟩
+                 have ih := @eG.unique_nodes i_idx j_idx (by grind) (by grind) ne
+                 have lemi := List.getElem_set hi
+                 have lemj := List.getElem_set hj
+                 simp at h; rcases h with ⟨e1, e2, e3, e4, e5, e6, e7, e8, e9, e10⟩; subst e5; subst e6; subst e3
+                 cases Nat.decEq ip1 i_idx
+                 case _ ni =>
+                   cases Nat.decEq ip1 j_idx
+                   case _ nj =>
+                    rw[ite_cond_eq_false (h := by grind)] at lemi
+                    rw[ite_cond_eq_false (h := by grind)] at lemj
+                    rw[lemi, lemj]; apply ih
+                   case _ nj =>
+                    rw[ite_cond_eq_false (h := by grind)] at lemi
+                    rw[ite_cond_eq_true (h := by grind)] at lemj
+                    subst nj; rw[lemj, lemi]; simp only [new_node, EqGraphNode.ty]; rw[h3] at ih
+                    apply ih
+                 case _ ni =>
+                  subst ni;
+                  rw[ite_cond_eq_true (h := by grind)] at lemi
+                  rw[ite_cond_eq_false (h := by grind)] at lemj
+                  rw[lemi, lemj]; simp only [new_node, EqGraphNode.ty]; rw[h3] at ih; apply ih
+              /-, equiv_class_count_ub := sorry
+              , equiv_class_count_lb := by intro h; sorry -/
               }
         else none
+    | _, _ => none
   | _, _ => none
-
-
-def EqGraph.equiv_class_count {G : GlobalEnv} {Δ : KindEnv} {Γ : TyEnv} (eG : EqGraph G Δ Γ) : Nat
-  := (eG.nodes.filter (λ n => n.parent_ty == n.ty)).length
 
 theorem EqGraph.union_equiv_class_count {G : GlobalEnv} {wf : ⊢ G} {Δ : KindEnv} {Γ : TyEnv}
   {eG eG' : EqGraph G Δ Γ} {K : Kind}
-  {T1 : Ty} {T2 : Ty} {t : Term} {j : G&Δ, Γ ⊢ t : (T1 ~[K]~ T2)} :
-  eG.union (G := G) (Δ := Δ) (Γ := Γ) (wf := wf) K T1 T2 t j = some eG' ->
+  {T1 : Ty} {T2 : Ty} {t : Term} {j : G&Δ, Γ ⊢ t : (T1 ~[K]~ T2)} (inv : eG.equiv_class_count > 0):
+  eG.union (wf := wf) K T1 T2 t j = some eG' ->
   eG'.equiv_class_count < eG.equiv_class_count
   := by
   intro h
@@ -658,43 +794,17 @@ theorem EqGraph.union_equiv_class_count {G : GlobalEnv} {wf : ⊢ G} {Δ : KindE
   rw[Option.bind_eq_some_iff] at h; rcases h with ⟨i1, h1, h⟩
   rw[Option.bind_eq_some_iff] at h; rcases h with ⟨i2, h2, h⟩
   split at h
-  case _ n1 n2 e1 e2 =>
-    rw[Option.bind_eq_some_iff] at h; rcases h with ⟨⟨ip1, pT1, K1, _, _⟩, h3, h⟩
+  · rw[Option.bind_eq_some_iff] at h; rcases h with ⟨⟨ip1, pT1, K1, _, _⟩, h3, h⟩
     rw[Option.bind_eq_some_iff] at h; rcases h with ⟨⟨ip2, pT2, K2, _, _⟩, h4, h⟩
-    rw[Option.bind_eq_some_iff] at h; rcases h with ⟨pn1, h5, h⟩
-    rw[Option.bind_eq_some_iff] at h; rcases h with ⟨pn2, h6, h⟩
-    simp at h; rcases h with ⟨ne, h⟩
-    simp at h5 h6
-    have len_lem : eG.nodes.length > 0 := by
-      induction eG.nodes
-      · sorry
-      · simp at *
+    simp at h
     split at h
-    case _ d =>
-      simp at d;
-      rcases d with ⟨e1, e2, e3, e4, e5, e6, e7, e8, e9, e10⟩; subst e6; subst pT1; subst pT2; subst K2; subst K
-      simp at h
-      simp only [<-h, EqGraph.equiv_class_count];
-      rw[List.filter_set_length e2]; simp; split
-      case _ d =>
-        exfalso; simp at d;
-        have lem := eG.unique_nodes (i := ip1) (j := ip2) (by grind) e2 ne;
-        rw[List.getElem?_eq_getElem (by grind)] at h6;
-        rw[List.getElem?_eq_getElem (by grind)] at h5; simp at h6 h5; subst h6; subst h5;
-        simp at lem; apply lem d
-      case _ =>
-        sorry
-    case _ =>
-      split at h
-      case _ d =>
-        simp at d
-        rcases d with ⟨e1, e2, e3, e4, e5, e6, e7, e8, e9, e10⟩; subst e6; subst pT1; subst pT2; subst K2; subst K
-        simp at h
-        simp only [<-h, EqGraph.equiv_class_count];
-        sorry
-      case _ => cases h
-  case _ => cases h
-
+    · simp at h;
+      rcases h with ⟨ne, h⟩
+      split at h <;> simp at h
+      · rw[<-h]; simp; omega
+      · rcases h with ⟨_, h⟩; rw[<-h]; simp; omega
+    · cases h
+  · cases h
 
 partial def EqGraph.process_equation (G : GlobalEnv) (wf : ⊢ G) (Δ : KindEnv) (Γ : TyEnv) (eG : EqGraph G Δ Γ) (K : Kind) :
   (T1 : Ty) -> (T2 : Ty) -> ((t : Term) ×' G&Δ, Γ ⊢ t : (T1 ~[K]~ T2)) -> Option (EqGraph G Δ Γ)
@@ -740,11 +850,12 @@ partial def EqGraph.process_equation (G : GlobalEnv) (wf : ⊢ G) (Δ : KindEnv)
   let clsT2 := eG.get_eq_class wf T2
   let p := (clsT1.flatMap (λ a => List.map (Prod.mk a) clsT2)).filter (λ (n1, n2) => n1.ty != T1 || n2.ty != T2)
   let eG' <- p.foldlM (λ acc (n1, n2) => do
-      let ⟨_, pT1, K1, η1, j1⟩ <- eG.get_rep wf n1.ty
-      let ⟨_, pT2, K2, η2, j2⟩ <- eG.get_rep wf n2.ty
+      let ⟨_, pT1, K1, η1, j1⟩ <- acc.get_rep wf n1.ty
+      let ⟨_, pT2, K2, η2, j2⟩ <- acc.get_rep wf n2.ty
       if h : K1 == K2 && (K == K1 && (Kp1 == K && (Kp2 == K && (rep_T1 == pT1 && rep_T2 == pT2))))
         then
-          by simp at h; rcases h with ⟨e1, e2, e3, e4, e5, e6⟩; subst K1; subst K2; subst Kp1; subst Kp2; subst pT1; subst pT2
+          by simp at h; rcases h with ⟨e1, e2, e3, e4, e5, e6⟩;
+             subst K1; subst K2; subst Kp1; subst Kp2; subst pT1; subst pT2
              apply do
                -- η1 ; symm c1; c; c2; symm η2
                let ⟨symm_η2, symm_j2⟩ := EqGraph.symm G wf Δ Γ η2 K n2.ty rep_T2 j2
@@ -764,6 +875,7 @@ partial def EqGraph.process_equation (G : GlobalEnv) (wf : ⊢ G) (Δ : KindEnv)
   if ip1 == ip2 && pT1 == pT2 then return eG'
   else eG'.union (wf := wf) K T1 T2 c j3
 
+
 def EqGraph.ask (G : GlobalEnv) (wf : ⊢ G) (Δ : KindEnv) (Γ : TyEnv) (eG : EqGraph G Δ Γ) (K : Kind) :
   (T1 : Ty) -> (T2 : Ty) -> Option ((t : Term) ×' G&Δ, Γ ⊢ t : (T1 ~[K]~ T2))
  | .app A1 B1, .app A2 B2 => do
@@ -778,7 +890,7 @@ def EqGraph.ask (G : GlobalEnv) (wf : ⊢ G) (Δ : KindEnv) (Γ : TyEnv) (eG : E
        by simp at h; rcases h with ⟨e1, e2, e3, e4, e5⟩; subst e1; subst e2; subst e3; subst e4; subst e5
           apply do let ⟨c1, j1⟩ <- EqGraph.ask G wf Δ Γ eG (K1a -:> K) A1 A2
                    let ⟨c2, j2⟩ <- EqGraph.ask G wf Δ Γ eG K1a B1 B2
-                   return EqGraph.appc G Δ Γ c1 c2 K1a K A1 A2 B1 B2 j1 j2
+                   return EqGraph.appc G wf Δ Γ c1 c2 K1a K A1 A2 B1 B2 j1 j2
      else none
    | _, _, _, _ => none
 -- TODO : Ditto for -:>
